coq-osiris/theories/program_logic/basic_rules.v
@@ -797,7 +797,7 @@ Section ewp_rules.
   Lemma ewp_wrap_shallow {B Y} E l η bs (k: _ -> micro B Y) φ ψ :
     (∀ l',
       l'↦
-        (K (λ o, Handle (stop CResume (l, o)) (λ o, shallow_match η o bs bs))) -∗
+        (K (λ o, Handle (stop CResume (l, o)) (shallow_eval_branches η bs bs))) -∗
      ▷ EWP (continue k l') @ E <| ψ |> {{ φ }}) -∗
     EWP (Stop CWrap (false, l, η, bs) k) @ E <| ψ |> {{ φ }}.
   Proof.
